@prefix : <http://linked.data.gov.au/def/geoadminfeatures#> .
@prefix dct: <http://purl.org/dc/terms/> .
@prefix geo: <http://www.opengis.net/ont/geosparql#> .
@prefix owl: <http://www.w3.org/2002/07/owl#> .
@prefix rdf: <http://www.w3.org/1999/02/22-rdf-syntax-ns#> .
@prefix sdo: <https://schema.org/> .
@prefix xml: <http://www.w3.org/XML/1998/namespace> .
@prefix xsd: <http://www.w3.org/2001/XMLSchema#> .
@prefix doap: <http://usefulinc.com/ns/doap#> .
@prefix loci: <http://linked.data.gov.au/def/loci#> .
@prefix prov: <http://www.w3.org/ns/prov#> .
@prefix rdfs: <http://www.w3.org/2000/01/rdf-schema#> .
@prefix skos: <http://www.w3.org/2004/02/skos/core#> .
@prefix geoaf: <http://linked.data.gov.au/def/geoadminfeatures#> .
@prefix schema: <http://schema.org/> .
@prefix dcterms: <http://purl.org/dc/terms/> .
@base <http://linked.data.gov.au/def/geoadminfeatures> .

<http://linked.data.gov.au/def/geoadminfeatures> rdf:type owl:Ontology ;
                                                  owl:imports <http://www.opengis.net/ont/geosparql> ;
                                                  dcterms:contributor [ rdf:type sdo:Person ;
                                                                        sdo:affiliation <http://linked.data.gov.au/org/gsq> ;
                                                                        sdo:email <mailto:andrew.isles@dnrme.qld.gov.au> ;
                                                                        sdo:name "Andrew Isles"
                                                                      ] ;
                                                  dcterms:creator [ rdf:type sdo:Person ;
                                                                    sdo:affiliation [ rdf:type sdo:Organization ;
                                                                                      sdo:identifier <https://surroundaustralia.com> ;
                                                                                      sdo:name "SURROUND Australia Pty Ltd"
                                                                                    ] ;
                                                                    sdo:email <mailto:nicholas.car@surroundaustralia.com> ;
                                                                    sdo:identifier <http://orcid.org/0000-0002-8742-7730> ;
                                                                    sdo:name "Nicholas J. Car"
                                                                  ] ,
                                                                  [ rdf:type sdo:Person ;
                                                                    sdo:affiliation <http://linked.data.gov.au/org/gsq> ;
                                                                    sdo:email <mailto:john.mckellar@dnrme.qld.gov.au> ;
                                                                    sdo:name "John McKellar"
                                                                  ] ;
                                                  dcterms:description """This ontology describes classes of geological and administrative feature relevant to the duties of the Geological Survey of Queensland.

As subclasses of the GeoSPARQL Ontology's `Feature` class, this ontology defines `Geological Feature` and `Administrative Feature`. Multiple subclasses of those two main classes are also defined.

Most of the subclasses of `Geological Feature` defined here are not disjoint with other subclasses of it in recognition of the fact that a real-world `Feature` may be classed in multiple ways. `Administrative Feature` subclasses, however, are all disjoint having been defined disjointly by people.

References to and positioning of other Features defined elsewhere are made, such as placing the HY_Features model's `Catchment` and `CatchmentAggregate` classes as subclasses of this ontology's `Basin` class (a subclass of `Geological Feature`). As a result, the classes of object within the LocI project's Geofabric dataset can be related to objects classified using this ontology."""@en ;
                                                  dcterms:hasVersion 0.5 ;
                                                  dcterms:modified "2019-10-08"^^xsd:date ;
                                                  dcterms:publisher <http://linked.data.gov.au/org/gsq> ;
                                                  dcterms:title "Geological and Administrative Features Ontology"@en ;
                                                  prov:wasGeneratedBy [ rdf:type doap:Project ,
                                                                                 prov:Activity ;
                                                                        doap:repository <https://github.com/geological-survey-of-queensland/gsq-geoadminfeatures-ont>
                                                                      ] .

#################################################################
#    Annotation properties
#################################################################

###  http://usefulinc.com/ns/doap#repository
doap:repository rdf:type owl:AnnotationProperty .


###  http://www.w3.org/ns/prov#wasGeneratedBy
prov:wasGeneratedBy rdf:type owl:AnnotationProperty .


###  https://schema.org/affiliation
sdo:affiliation rdf:type owl:AnnotationProperty .


###  https://schema.org/email
sdo:email rdf:type owl:AnnotationProperty .


###  https://schema.org/identifier
sdo:identifier rdf:type owl:AnnotationProperty .


###  https://schema.org/name
sdo:name rdf:type owl:AnnotationProperty .


#################################################################
#    Classes
#################################################################

###  http://linked.data.gov.au/def/geoadminfeatures#AdministrativeFeature
geoaf:AdministrativeFeature rdf:type owl:Class ;
                            rdfs:subClassOf geo:Feature ;
                            owl:disjointWith geoaf:GeologicalFeature ;
                            skos:definition "An Administrative Feature is a geo:Feature that is defined by adminstrative processes such as legislation, regulation, policy or procedure."@en ;
                            skos:prefLabel "Administrative feature" .


###  http://linked.data.gov.au/def/geoadminfeatures#Block
geoaf:Block rdf:type owl:Class ;
            rdfs:subClassOf geoaf:AdministrativeFeature ;
            skos:definition "A Block is an administrative division of the State of Queensland that is used for tenure management. A Block is defined as five minutes of latitude by five minutes of longitude. Blocks are grouped by 1:1,000,000 map sheet areas, the names of which provide the containing Blocks with a four letter prefix (e.g. Clermont 1:1,000,000 provides CLER). Each sheet area contains 3456 Blocks, with the Blocks numbered between 1 and 3456 inclusive. A Block is divided into 25 Sub-Blocks."@en ;
            skos:prefLabel "Block" .


###  http://linked.data.gov.au/def/geoadminfeatures#GeoResourceAccumulation
geoaf:GeoResourceAccumulation rdf:type owl:Class ;
                              rdfs:subClassOf geoaf:GeologicalFeature ;
                              skos:definition "Georesource accumulations are naturally occurring masses, volumes or concentrations of geological materials that have existing or potential economic value. These resources may include, but are not limited to, minerals (including coal), hydrocarbons, quarry resources and groundwater."@en ;
                              skos:prefLabel "GeoResource Accumulation" .


###  http://linked.data.gov.au/def/geoadminfeatures#GeologicalFeature
geoaf:GeologicalFeature rdf:type owl:Class ;
                        rdfs:subClassOf geo:Feature ;
                        skos:definition "A Geological Feature is a geospatial Feature that is a result of geological processes."@en ;
                        skos:prefLabel "Geological Feature" .


###  http://linked.data.gov.au/def/geoadminfeatures#LithodemicFeature
geoaf:LithodemicFeature rdf:type owl:Class ;
                        rdfs:subClassOf geoaf:GeologicalFeature ;
                        owl:disjointWith geoaf:StratigraphicFeature ;
                        skos:definition "A Lithodemic Feature is a Geological Feature that was not created by sedimentation proceeses." ;
                        skos:prefLabel "Lithodemic Feature" .


###  http://linked.data.gov.au/def/geoadminfeatures#Permit
geoaf:Permit rdf:type owl:Class ;
             rdfs:subClassOf geoaf:AdministrativeFeature ;
             skos:definition "Permits are a license granted over a spatial region within the State of Queensland. Permits govern the activities which can be conducted upon them. Activities include exploration, development, and extraction of a specific commodity or commodities."@en ;
             skos:prefLabel "Permit" .


###  http://linked.data.gov.au/def/geoadminfeatures#StratigraphicFeature
geoaf:StratigraphicFeature rdf:type owl:Class ;
                           rdfs:subClassOf geoaf:GeologicalFeature ;
                           skos:definition "Stratigraphic Features embrace Stratigraphic Units, which are units of rock and/or sediment that conform to the Law of Superposition (e.g. lithostratigraphic units, biostratigraphic units, chronostratigraphic units), and Stratigraphic Events which reflect physical, chemical and biological events that left identifiable, widespread, if not worldwide, traces or markers in the sedimentary or extrusive igneous record (ICS; Kumpulainen, R.A., 2016)."@en ;
                           skos:prefLabel "Stratigraphic Feature" .


###  http://linked.data.gov.au/def/geoadminfeatures#SubBlock
geoaf:SubBlock rdf:type owl:Class ;
               rdfs:subClassOf geoaf:AdministrativeFeature ,
                               [ rdf:type owl:Restriction ;
                                 owl:onProperty geo:sfWithin ;
                                 owl:qualifiedCardinality "1"^^xsd:nonNegativeInteger ;
                                 owl:onClass geoaf:Block
                               ] ;
               skos:definition "A Sub-Block is an administrative sub-division of a Block. Each Block is divided into 25 Sub-Blocks. A Sub-Block is defined as one minute of latitude by one minute of longitude. The Sub-Blocks are prefixed with their corresponding Block name and are labelled from A to Z, excluding I. Labels are allocated from left to right, top to bottom, starting from the northwest corner."@en ;
               skos:prefLabel "Sub-Block" .


###  http://linked.data.gov.au/def/geoadminfeatures#TechtonicAndStructuralFrameworkFeature
geoaf:TechtonicAndStructuralFrameworkFeature rdf:type owl:Class ;
                                             rdfs:subClassOf geoaf:GeologicalFeature ;
                                             skos:definition "A Tectonic and Structural Framework Feature is a Tectonic, Tectonostratigraphic or Structural element. Tectonic Elements include cratons, orogens, provinces and sedimentary basins; Tectonostratigraphic Elements include nappes and klippen; and Structural Elements include synclines, anticlines, faults and half-grabens."@en ;
                                             skos:prefLabel "Techtonic And Structural Framework Feature" .


###  http://usefulinc.com/ns/doap#Project
doap:Project rdf:type owl:Class .


###  http://www.w3.org/ns/prov#Activity
prov:Activity rdf:type owl:Class .


###  https://schema.org/Organization
sdo:Organization rdf:type owl:Class .


###  https://schema.org/Person
sdo:Person rdf:type owl:Class .


#################################################################
#    Individuals
#################################################################

###  http://linked.data.gov.au/org/gsq
<http://linked.data.gov.au/org/gsq> rdf:type owl:NamedIndividual ,
                                             sdo:Organization ;
                                    sdo:identifier <http://linked.data.gov.au/org/gsq> ;
                                    sdo:name "Geological Survey of Queensland" .


[ rdf:type sdo:Person ;
  sdo:affiliation [ rdf:type sdo:Organization ;
                    sdo:identifier <https://surroundaustralia.com> ;
                    sdo:name "SURROUND Australia Pty Ltd"
                  ] ;
  sdo:email <mailto:nicholas.car@surroundaustralia.com> ;
  sdo:identifier <http://orcid.org/0000-0002-8742-7730> ;
  sdo:name "Nicholas J. Car"
] .

[ rdf:type sdo:Person ;
   sdo:affiliation <http://linked.data.gov.au/org/gsq> ;
   sdo:email <mailto:john.mckellar@dnrme.qld.gov.au> ;
   sdo:name "John McKellar"
 ] .

[ rdf:type sdo:Person ;
   sdo:affiliation <http://linked.data.gov.au/org/gsq> ;
   sdo:email <mailto:andrew.isles@dnrme.qld.gov.au> ;
   sdo:name "Andrew Isles"
 ] .

[ rdf:type doap:Project ,
            prov:Activity ;
   doap:repository <https://github.com/geological-survey-of-queensland/gsq-geoadminfeatures-ont>
 ] .

###  Generated by the OWL API (version 4.5.9.2019-02-01T07:24:44Z) https://github.com/owlcs/owlapi
