@prefix : <http://linked.data.gov.au/def/geoadminfeatures#> .
@prefix dct: <http://purl.org/dc/terms/> .
@prefix owl: <http://www.w3.org/2002/07/owl#> .
@prefix rdf: <http://www.w3.org/1999/02/22-rdf-syntax-ns#> .
@prefix xml: <http://www.w3.org/XML/1998/namespace> .
@prefix xsd: <http://www.w3.org/2001/XMLSchema#> .
@prefix doap: <http://usefulinc.com/ns/doap#> .
@prefix prov: <http://www.w3.org/ns/prov#> .
@prefix rdfs: <http://www.w3.org/2000/01/rdf-schema#> .
@prefix skos: <http://www.w3.org/2004/02/skos/core#> .
@prefix schema: <https://schema.org/> .
@base <http://linked.data.gov.au/def/geoadminfeatures> .

<http://linked.data.gov.au/def/geoadminfeatures> rdf:type owl:Ontology ;
                                                  owl:imports <http://www.opengis.net/ont/geosparql> ;
                                                  dct:contributor [ rdf:type sdo:Person ;
                                                                        sdo:affiliation <http://linked.data.gov.au/org/gsq> ;
                                                                        sdo:email <mailto:andrew.isles@dnrme.qld.gov.au> ;
                                                                        sdo:name "Andrew Isles"
                                                                      ] ;
                                                  dct:creator [ rdf:type sdo:Person ;
                                                                    sdo:affiliation [ rdf:type sdo:Organization ;
                                                                                      sdo:identifier <https://surroundaustralia.com> ;
                                                                                      sdo:name "SURROUND Australia Pty Ltd"
                                                                                    ] ;
                                                                    sdo:email <mailto:nicholas.car@surroundaustralia.com> ;
                                                                    sdo:identifier <http://orcid.org/0000-0002-8742-7730> ;
                                                                    sdo:name "Nicholas J. Car"
                                                                  ] ,
                                                                  [ rdf:type sdo:Person ;
                                                                    sdo:affiliation <http://linked.data.gov.au/org/gsq> ;
                                                                    sdo:email <mailto:john.mckellar@dnrme.qld.gov.au> ;
                                                                    sdo:name "John McKellar"
                                                                  ] ;
                                                  dct:description """This ontology describes classes of geological and administrative feature relevant to the duties of the Geological Survey of Queensland.

As subclasses of the GeoSPARQL Ontology's `Feature` class, this ontology defines `Geological Feature` and `Administrative Feature`. Multiple subclasses of those two main classes are also defined.

Most of the subclasses of `Geological Feature` defined here are not disjoint with other subclasses of it in recognition of the fact that a real-world `Feature` may be classed in multiple ways. `Administrative Feature` subclasses, however, are all disjoint having been defined disjointly by people.

References to and positioning of other Features defined elsewhere are made, such as placing the HY_Features model's `Catchment` and `CatchmentAggregate` classes as subclasses of this ontology's `Basin` class (a subclass of `Geological Feature`). As a result, the classes of object within the LocI project's Geofabric dataset can be related to objects classified using this ontology."""@en ;
                                                  dct:hasVersion 0.5 ;
                                                  dct:modified "2019-10-08"^^xsd:date ;
                                                  dct:publisher <http://linked.data.gov.au/org/gsq> ;
                                                  dct:title "Geological and Administrative Features Ontology"@en ;
                                                  prov:wasGeneratedBy [ rdf:type doap:Project ,
                                                                                 prov:Activity ;
                                                                        doap:repository <https://github.com/geological-survey-of-queensland/gsq-geoadminfeatures-ont>
                                                                      ] .

#################################################################
#    Annotation properties
#################################################################

###  http://usefulinc.com/ns/doap#repository
doap:repository rdf:type owl:AnnotationProperty .


###  http://www.w3.org/2000/01/rdf-schema#prefLabel
rdfs:prefLabel rdf:type owl:AnnotationProperty .


###  http://www.w3.org/ns/prov#wasGeneratedBy
prov:wasGeneratedBy rdf:type owl:AnnotationProperty .


###  https://schema.org/affiliation
schema:affiliation rdf:type owl:AnnotationProperty .


###  https://schema.org/email
schema:email rdf:type owl:AnnotationProperty .


###  https://schema.org/identifier
schema:identifier rdf:type owl:AnnotationProperty .


###  https://schema.org/name
schema:name rdf:type owl:AnnotationProperty .


#################################################################
#    Classes
#################################################################

###  http://linked.data.gov.au/def/geoadminfeatures#AdministrativeFeature
:AdministrativeFeature rdf:type owl:Class ;
                       rdfs:subClassOf <http://www.opengis.net/ont/geosparql#Feature> ;
                       owl:disjointWith :GeologicalFeature ;
                       skos:definition "An Administrative Feature is a geo:Feature that is defined by adminstrative processes such as legislation, regulation, policy or procedure."@en ;
                       skos:prefLabel "Administrative feature" .


###  http://linked.data.gov.au/def/geoadminfeatures#Basin
:Basin rdf:type owl:Class ;
       rdfs:subClassOf :StructuralFrameworkFeature ;
       rdfs:prefLabel "Basin" ;
       skos:definition "A Basin is a Structural Framework Feature that is or was defined by hydrological processes. Basins are not necissarily any longer related to hydrological processes as they could have been created by hydrological actions long in the past and have been altered by other geological processes since."@en .


###  http://linked.data.gov.au/def/geoadminfeatures#Block
:Block rdf:type owl:Class ;
       rdfs:subClassOf :AdministrativeFeature ;
       rdfs:prefLabel "Block" ;
       skos:definition "A Block is an administrative division of the State of Queensland that is used for tenure management. A Block is defined as five minutes of latitude by five minutes of longitude. Blocks are grouped by 1:1,000,000 map sheet areas, the names of which provide the containing Blocks with a four letter prefix (e.g. Clermont 1:1,000,000 provides CLER). Each sheet area contains 3456 Blocks, with the Blocks numbered between 1 and 3456 inclusive. A Block is divided into 25 Sub-Blocks."@en ,
                       """Blocks are Administrative Features that are defined for the adminstration of mining leases.
Individual Blocks are defined by the Queensland Department of Natural Resources, Mines and Energy's Geological Survey of Queensland's Permit Administration unit."""@en ;
       skos:prefLabel "Block" .


###  http://linked.data.gov.au/def/geoadminfeatures#Craton
:Craton rdf:type owl:Class ;
        rdfs:subClassOf :StructuralFrameworkFeature ;
        rdfs:prefLabel "Craton" .


###  http://linked.data.gov.au/def/geoadminfeatures#GeoResourceAccumulation
:GeoResourceAccumulation rdf:type owl:Class ;
                         rdfs:subClassOf :GeologicalFeature ;
                         skos:definition "Georesource accumulations are naturally occurring masses, volumes or concentrations of geological materials that have existing or potential economic value. These resources may include, but are not limited to, minerals (including coal), hydrocarbons, quarry resources and groundwater."@en ;
                         skos:prefLabel "GeoResource Accumulation" .


###  http://linked.data.gov.au/def/geoadminfeatures#GeologicalFeature
:GeologicalFeature rdf:type owl:Class ;
                   rdfs:subClassOf <http://www.opengis.net/ont/geosparql#Feature> ;
                   skos:definition "A Geological Feature is a geospatial Feature that is a result of geological processes."@en ;
                   skos:prefLabel "Geological Feature" .


###  http://linked.data.gov.au/def/geoadminfeatures#GroundwaterBasin
:GroundwaterBasin rdf:type owl:Class ;
                  rdfs:subClassOf :Basin ;
                  rdfs:prefLabel "Groundwater Basin" ;
                  skos:definition "A Groundwater Basin is a subsurface, three-dimensional, water-storage system contained by porous sediments and/or sedimentary rocks comprising an aquifer or a succession of stacked aquifers that are separated by non-porous and generally impermeable sediments or rocks (termed acquitards or, if completely impermeable, aquicludes). Groundwater Basins have recharge and discharge zones, the latter where water flows back to the surface at springs or into rivers, lakes, etc."@en .


###  http://linked.data.gov.au/def/geoadminfeatures#LithodemicFeature
:LithodemicFeature rdf:type owl:Class ;
                   rdfs:subClassOf :GeologicalFeature ;
                   owl:disjointWith :StratigraphicFeature ;
                   skos:definition "A Lithodemic Feature is a Geological Feature that was not created by sedimentation proceeses." ;
                   skos:prefLabel "Lithodemic Feature" .


###  http://linked.data.gov.au/def/geoadminfeatures#Orogen
:Orogen rdf:type owl:Class ;
        rdfs:subClassOf :StructuralFrameworkFeature ;
        rdfs:prefLabel "Orogen" .


###  http://linked.data.gov.au/def/geoadminfeatures#Permit
:Permit rdf:type owl:Class ;
        rdfs:subClassOf :AdministrativeFeature ;
        rdfs:prefLabel "Permit" ;
        skos:definition "Permits are a license granted over a spatial region within the State of Queensland. Permits govern the activities which can be conducted upon them. Activities include exploration, development, and extraction of a specific commodity or commodities."@en ;
        skos:prefLabel "Permit" .


###  http://linked.data.gov.au/def/geoadminfeatures#Province
:Province rdf:type owl:Class ;
          rdfs:subClassOf :StructuralFrameworkFeature ;
          rdfs:prefLabel "Province" .


###  http://linked.data.gov.au/def/geoadminfeatures#ResourceAccumulationFeature
:ResourceAccumulationFeature rdf:type owl:Class ;
                             rdfs:subClassOf :GeologicalFeature ;
                             skos:prefLabel "Resource Accumulation Feature" .


###  http://linked.data.gov.au/def/geoadminfeatures#SedimentaryBasin
:SedimentaryBasin rdf:type owl:Class ;
                  rdfs:subClassOf :Basin ;
                  rdfs:prefLabel "Sedimentary Basin" ;
                  skos:definition """A Sedimentary Basin comprises a three-dimensional region in which sediments accumulate or have accumulated from a range of varying geological/tectonic causes.
Present-day sedimentary basins include the internal-draining Lake Eyre Basin (central Australia), but, from a geological perspective, primary focus is given to resource-rich, Sedimentary Basins that formed, and were subsequently terminated by a causative event (e.g., tectonic uplift), at varying times in the geological past."""@en .


###  http://linked.data.gov.au/def/geoadminfeatures#StratigraphicFeature
:StratigraphicFeature rdf:type owl:Class ;
                      rdfs:subClassOf :GeologicalFeature ;
                      skos:definition "Stratigraphic Features embrace Stratigraphic Units, which are units of rock and/or sediment that conform to the Law of Superposition (e.g. lithostratigraphic units, biostratigraphic units, chronostratigraphic units), and Stratigraphic Events which reflect physical, chemical and biological events that left identifiable, widespread, if not worldwide, traces or markers in the sedimentary or extrusive igneous record (ICS; Kumpulainen, R.A., 2016)."@en ;
                      skos:prefLabel "Stratigraphic Feature" .


###  http://linked.data.gov.au/def/geoadminfeatures#StructuralFrameworkFeature
:StructuralFrameworkFeature rdf:type owl:Class ;
                            rdfs:subClassOf :GeologicalFeature ;
                            skos:prefLabel "Structural Framework Feature" .


###  http://linked.data.gov.au/def/geoadminfeatures#SubBlock
:SubBlock rdf:type owl:Class ;
          rdfs:subClassOf :AdministrativeFeature ,
                          [ rdf:type owl:Restriction ;
                            owl:onProperty <http://www.opengis.net/ont/geosparql#sfWithin> ;
                            owl:qualifiedCardinality "1"^^xsd:nonNegativeInteger ;
                            owl:onClass :Block
                          ] ;
          rdfs:prefLabel "Sub-Block" ;
          skos:definition """A Sub-Block is an Adminstrative Feature that is always fully contained within a larger Block.
Individual Sub-Blocks are defined by the Queensland Department of Natural Resources, Mines and Energy's Geological Survey of Queensland's Permit Administration unit."""@en ,
                          "A Sub-Block is an administrative sub-division of a Block. Each Block is divided into 25 Sub-Blocks. A Sub-Block is defined as one minute of latitude by one minute of longitude. The Sub-Blocks are prefixed with their corresponding Block name and are labelled from A to Z, excluding I. Labels are allocated from left to right, top to bottom, starting from the northwest corner."@en ;
          skos:prefLabel "Sub-Block" .


###  http://linked.data.gov.au/def/geoadminfeatures#SubProvince
:SubProvince rdf:type owl:Class ;
             rdfs:subClassOf :StructuralFrameworkFeature ,
                             [ rdf:type owl:Restriction ;
                               owl:onProperty <http://www.opengis.net/ont/geosparql#sfWithin> ;
                               owl:qualifiedCardinality "1"^^xsd:nonNegativeInteger ;
                               owl:onClass :Province
                             ] ;
             rdfs:prefLabel "Sub-Province" .


###  http://linked.data.gov.au/def/geoadminfeatures#TechtonicAndStructuralFrameworkFeature
:TechtonicAndStructuralFrameworkFeature rdf:type owl:Class ;
                                        rdfs:subClassOf :GeologicalFeature ;
                                        skos:definition "A Tectonic and Structural Framework Feature is a Tectonic, Tectonostratigraphic or Structural element. Tectonic Elements include cratons, orogens, provinces and sedimentary basins; Tectonostratigraphic Elements include nappes and klippen; and Structural Elements include synclines, anticlines, faults and half-grabens."@en ;
                                        skos:prefLabel "Techtonic And Structural Framework Feature" .
